Remove motive from the syntax and update preservation

syntax.sig
@@ -9,7 +9,7 @@ tUniv : nat -> tm
 tVoid : tm
 tAbsurd : tm -> tm
 tEq : T -> tm -> tm -> tm -> tm
-tJ : (tm -> tm -> tm) -> tm -> tm -> tm
+tJ : tm -> tm -> tm
 tRefl : tm
 tSig : T -> tm -> (tm -> tm) -> tm
 tPack : T -> tm -> tm -> tm
