theories/Autosubst2/syntax.v
@@ -18,7 +18,7 @@ Inductive tm  : Type :=
   | tVoid : tm 
   | tAbsurd : ( tm   ) -> tm 
   | tEq : ( T   ) -> ( tm   ) -> ( tm   ) -> ( tm   ) -> tm 
-  | tJ : ( tm   ) -> ( tm   ) -> ( tm   ) -> tm 
+  | tJ : ( tm   ) -> ( tm   ) -> tm 
   | tRefl : tm 
   | tSig : ( T   ) -> ( tm   ) -> ( tm   ) -> tm 
   | tPack : ( T   ) -> ( tm   ) -> ( tm   ) -> tm 
@@ -45,7 +45,7 @@ Proof. congruence. Qed.
 Lemma congr_tEq  { s0 : T   } { s1 : tm   } { s2 : tm   } { s3 : tm   } { t0 : T   } { t1 : tm   } { t2 : tm   } { t3 : tm   } (H1 : s0 = t0) (H2 : s1 = t1) (H3 : s2 = t2) (H4 : s3 = t3) : tEq  s0 s1 s2 s3 = tEq  t0 t1 t2 t3 .
 Proof. congruence. Qed.
 
-Lemma congr_tJ  { s0 : tm   } { s1 : tm   } { s2 : tm   } { t0 : tm   } { t1 : tm   } { t2 : tm   } (H1 : s0 = t0) (H2 : s1 = t1) (H3 : s2 = t2) : tJ  s0 s1 s2 = tJ  t0 t1 t2 .
+Lemma congr_tJ  { s0 : tm   } { s1 : tm   } { t0 : tm   } { t1 : tm   } (H1 : s0 = t0) (H2 : s1 = t1) : tJ  s0 s1 = tJ  t0 t1 .
 Proof. congruence. Qed.
 
 Lemma congr_tRefl  : tRefl  = tRefl  .
@@ -73,7 +73,7 @@ Fixpoint ren_tm   (xitm : ( fin ) -> fin) (s : tm ) : tm  :=
     | tVoid   => tVoid 
     | tAbsurd  s0 => tAbsurd  ((ren_tm xitm) s0)
     | tEq  s0 s1 s2 s3 => tEq  ((fun x => x) s0) ((ren_tm xitm) s1) ((ren_tm xitm) s2) ((ren_tm xitm) s3)
-    | tJ  s0 s1 s2 => tJ  ((ren_tm (upRen_tm_tm (upRen_tm_tm xitm))) s0) ((ren_tm xitm) s1) ((ren_tm xitm) s2)
+    | tJ  s0 s1 => tJ  ((ren_tm xitm) s0) ((ren_tm xitm) s1)
     | tRefl   => tRefl 
     | tSig  s0 s1 s2 => tSig  ((fun x => x) s0) ((ren_tm xitm) s1) ((ren_tm (upRen_tm_tm xitm)) s2)
     | tPack  s0 s1 s2 => tPack  ((fun x => x) s0) ((ren_tm xitm) s1) ((ren_tm xitm) s2)
@@ -93,7 +93,7 @@ Fixpoint subst_tm   (sigmatm : ( fin ) -> tm ) (s : tm ) : tm  :=
     | tVoid   => tVoid 
     | tAbsurd  s0 => tAbsurd  ((subst_tm sigmatm) s0)
     | tEq  s0 s1 s2 s3 => tEq  ((fun x => x) s0) ((subst_tm sigmatm) s1) ((subst_tm sigmatm) s2) ((subst_tm sigmatm) s3)
-    | tJ  s0 s1 s2 => tJ  ((subst_tm (up_tm_tm (up_tm_tm sigmatm))) s0) ((subst_tm sigmatm) s1) ((subst_tm sigmatm) s2)
+    | tJ  s0 s1 => tJ  ((subst_tm sigmatm) s0) ((subst_tm sigmatm) s1)
     | tRefl   => tRefl 
     | tSig  s0 s1 s2 => tSig  ((fun x => x) s0) ((subst_tm sigmatm) s1) ((subst_tm (up_tm_tm sigmatm)) s2)
     | tPack  s0 s1 s2 => tPack  ((fun x => x) s0) ((subst_tm sigmatm) s1) ((subst_tm sigmatm) s2)
@@ -116,7 +116,7 @@ Fixpoint idSubst_tm  (sigmatm : ( fin ) -> tm ) (Eqtm : forall x, sigmatm x = (v
     | tVoid   => congr_tVoid 
     | tAbsurd  s0 => congr_tAbsurd ((idSubst_tm sigmatm Eqtm) s0)
     | tEq  s0 s1 s2 s3 => congr_tEq eq_refl ((idSubst_tm sigmatm Eqtm) s1) ((idSubst_tm sigmatm Eqtm) s2) ((idSubst_tm sigmatm Eqtm) s3)
-    | tJ  s0 s1 s2 => congr_tJ ((idSubst_tm (up_tm_tm (up_tm_tm sigmatm)) (upId_tm_tm (_) (upId_tm_tm (_) Eqtm))) s0) ((idSubst_tm sigmatm Eqtm) s1) ((idSubst_tm sigmatm Eqtm) s2)
+    | tJ  s0 s1 => congr_tJ ((idSubst_tm sigmatm Eqtm) s0) ((idSubst_tm sigmatm Eqtm) s1)
     | tRefl   => congr_tRefl 
     | tSig  s0 s1 s2 => congr_tSig eq_refl ((idSubst_tm sigmatm Eqtm) s1) ((idSubst_tm (up_tm_tm sigmatm) (upId_tm_tm (_) Eqtm)) s2)
     | tPack  s0 s1 s2 => congr_tPack eq_refl ((idSubst_tm sigmatm Eqtm) s1) ((idSubst_tm sigmatm Eqtm) s2)
@@ -139,7 +139,7 @@ Fixpoint extRen_tm   (xitm : ( fin ) -> fin) (zetatm : ( fin ) -> fin) (Eqtm : f
     | tVoid   => congr_tVoid 
     | tAbsurd  s0 => congr_tAbsurd ((extRen_tm xitm zetatm Eqtm) s0)
     | tEq  s0 s1 s2 s3 => congr_tEq eq_refl ((extRen_tm xitm zetatm Eqtm) s1) ((extRen_tm xitm zetatm Eqtm) s2) ((extRen_tm xitm zetatm Eqtm) s3)
-    | tJ  s0 s1 s2 => congr_tJ ((extRen_tm (upRen_tm_tm (upRen_tm_tm xitm)) (upRen_tm_tm (upRen_tm_tm zetatm)) (upExtRen_tm_tm (_) (_) (upExtRen_tm_tm (_) (_) Eqtm))) s0) ((extRen_tm xitm zetatm Eqtm) s1) ((extRen_tm xitm zetatm Eqtm) s2)
+    | tJ  s0 s1 => congr_tJ ((extRen_tm xitm zetatm Eqtm) s0) ((extRen_tm xitm zetatm Eqtm) s1)
     | tRefl   => congr_tRefl 
     | tSig  s0 s1 s2 => congr_tSig eq_refl ((extRen_tm xitm zetatm Eqtm) s1) ((extRen_tm (upRen_tm_tm xitm) (upRen_tm_tm zetatm) (upExtRen_tm_tm (_) (_) Eqtm)) s2)
     | tPack  s0 s1 s2 => congr_tPack eq_refl ((extRen_tm xitm zetatm Eqtm) s1) ((extRen_tm xitm zetatm Eqtm) s2)
@@ -162,7 +162,7 @@ Fixpoint ext_tm   (sigmatm : ( fin ) -> tm ) (tautm : ( fin ) -> tm ) (Eqtm : fo
     | tVoid   => congr_tVoid 
     | tAbsurd  s0 => congr_tAbsurd ((ext_tm sigmatm tautm Eqtm) s0)
     | tEq  s0 s1 s2 s3 => congr_tEq eq_refl ((ext_tm sigmatm tautm Eqtm) s1) ((ext_tm sigmatm tautm Eqtm) s2) ((ext_tm sigmatm tautm Eqtm) s3)
-    | tJ  s0 s1 s2 => congr_tJ ((ext_tm (up_tm_tm (up_tm_tm sigmatm)) (up_tm_tm (up_tm_tm tautm)) (upExt_tm_tm (_) (_) (upExt_tm_tm (_) (_) Eqtm))) s0) ((ext_tm sigmatm tautm Eqtm) s1) ((ext_tm sigmatm tautm Eqtm) s2)
+    | tJ  s0 s1 => congr_tJ ((ext_tm sigmatm tautm Eqtm) s0) ((ext_tm sigmatm tautm Eqtm) s1)
     | tRefl   => congr_tRefl 
     | tSig  s0 s1 s2 => congr_tSig eq_refl ((ext_tm sigmatm tautm Eqtm) s1) ((ext_tm (up_tm_tm sigmatm) (up_tm_tm tautm) (upExt_tm_tm (_) (_) Eqtm)) s2)
     | tPack  s0 s1 s2 => congr_tPack eq_refl ((ext_tm sigmatm tautm Eqtm) s1) ((ext_tm sigmatm tautm Eqtm) s2)
@@ -182,7 +182,7 @@ Fixpoint compRenRen_tm    (xitm : ( fin ) -> fin) (zetatm : ( fin ) -> fin) (rho
     | tVoid   => congr_tVoid 
     | tAbsurd  s0 => congr_tAbsurd ((compRenRen_tm xitm zetatm rhotm Eqtm) s0)
     | tEq  s0 s1 s2 s3 => congr_tEq eq_refl ((compRenRen_tm xitm zetatm rhotm Eqtm) s1) ((compRenRen_tm xitm zetatm rhotm Eqtm) s2) ((compRenRen_tm xitm zetatm rhotm Eqtm) s3)
-    | tJ  s0 s1 s2 => congr_tJ ((compRenRen_tm (upRen_tm_tm (upRen_tm_tm xitm)) (upRen_tm_tm (upRen_tm_tm zetatm)) (upRen_tm_tm (upRen_tm_tm rhotm)) (up_ren_ren (_) (_) (_) (up_ren_ren (_) (_) (_) Eqtm))) s0) ((compRenRen_tm xitm zetatm rhotm Eqtm) s1) ((compRenRen_tm xitm zetatm rhotm Eqtm) s2)
+    | tJ  s0 s1 => congr_tJ ((compRenRen_tm xitm zetatm rhotm Eqtm) s0) ((compRenRen_tm xitm zetatm rhotm Eqtm) s1)
     | tRefl   => congr_tRefl 
     | tSig  s0 s1 s2 => congr_tSig eq_refl ((compRenRen_tm xitm zetatm rhotm Eqtm) s1) ((compRenRen_tm (upRen_tm_tm xitm) (upRen_tm_tm zetatm) (upRen_tm_tm rhotm) (up_ren_ren (_) (_) (_) Eqtm)) s2)
     | tPack  s0 s1 s2 => congr_tPack eq_refl ((compRenRen_tm xitm zetatm rhotm Eqtm) s1) ((compRenRen_tm xitm zetatm rhotm Eqtm) s2)
@@ -205,7 +205,7 @@ Fixpoint compRenSubst_tm    (xitm : ( fin ) -> fin) (tautm : ( fin ) -> tm ) (th
     | tVoid   => congr_tVoid 
     | tAbsurd  s0 => congr_tAbsurd ((compRenSubst_tm xitm tautm thetatm Eqtm) s0)
     | tEq  s0 s1 s2 s3 => congr_tEq eq_refl ((compRenSubst_tm xitm tautm thetatm Eqtm) s1) ((compRenSubst_tm xitm tautm thetatm Eqtm) s2) ((compRenSubst_tm xitm tautm thetatm Eqtm) s3)
-    | tJ  s0 s1 s2 => congr_tJ ((compRenSubst_tm (upRen_tm_tm (upRen_tm_tm xitm)) (up_tm_tm (up_tm_tm tautm)) (up_tm_tm (up_tm_tm thetatm)) (up_ren_subst_tm_tm (_) (_) (_) (up_ren_subst_tm_tm (_) (_) (_) Eqtm))) s0) ((compRenSubst_tm xitm tautm thetatm Eqtm) s1) ((compRenSubst_tm xitm tautm thetatm Eqtm) s2)
+    | tJ  s0 s1 => congr_tJ ((compRenSubst_tm xitm tautm thetatm Eqtm) s0) ((compRenSubst_tm xitm tautm thetatm Eqtm) s1)
     | tRefl   => congr_tRefl 
     | tSig  s0 s1 s2 => congr_tSig eq_refl ((compRenSubst_tm xitm tautm thetatm Eqtm) s1) ((compRenSubst_tm (upRen_tm_tm xitm) (up_tm_tm tautm) (up_tm_tm thetatm) (up_ren_subst_tm_tm (_) (_) (_) Eqtm)) s2)
     | tPack  s0 s1 s2 => congr_tPack eq_refl ((compRenSubst_tm xitm tautm thetatm Eqtm) s1) ((compRenSubst_tm xitm tautm thetatm Eqtm) s2)
@@ -228,7 +228,7 @@ Fixpoint compSubstRen_tm    (sigmatm : ( fin ) -> tm ) (zetatm : ( fin ) -> fin)
     | tVoid   => congr_tVoid 
     | tAbsurd  s0 => congr_tAbsurd ((compSubstRen_tm sigmatm zetatm thetatm Eqtm) s0)
     | tEq  s0 s1 s2 s3 => congr_tEq eq_refl ((compSubstRen_tm sigmatm zetatm thetatm Eqtm) s1) ((compSubstRen_tm sigmatm zetatm thetatm Eqtm) s2) ((compSubstRen_tm sigmatm zetatm thetatm Eqtm) s3)
-    | tJ  s0 s1 s2 => congr_tJ ((compSubstRen_tm (up_tm_tm (up_tm_tm sigmatm)) (upRen_tm_tm (upRen_tm_tm zetatm)) (up_tm_tm (up_tm_tm thetatm)) (up_subst_ren_tm_tm (_) (_) (_) (up_subst_ren_tm_tm (_) (_) (_) Eqtm))) s0) ((compSubstRen_tm sigmatm zetatm thetatm Eqtm) s1) ((compSubstRen_tm sigmatm zetatm thetatm Eqtm) s2)
+    | tJ  s0 s1 => congr_tJ ((compSubstRen_tm sigmatm zetatm thetatm Eqtm) s0) ((compSubstRen_tm sigmatm zetatm thetatm Eqtm) s1)
     | tRefl   => congr_tRefl 
     | tSig  s0 s1 s2 => congr_tSig eq_refl ((compSubstRen_tm sigmatm zetatm thetatm Eqtm) s1) ((compSubstRen_tm (up_tm_tm sigmatm) (upRen_tm_tm zetatm) (up_tm_tm thetatm) (up_subst_ren_tm_tm (_) (_) (_) Eqtm)) s2)
     | tPack  s0 s1 s2 => congr_tPack eq_refl ((compSubstRen_tm sigmatm zetatm thetatm Eqtm) s1) ((compSubstRen_tm sigmatm zetatm thetatm Eqtm) s2)
@@ -251,7 +251,7 @@ Fixpoint compSubstSubst_tm    (sigmatm : ( fin ) -> tm ) (tautm : ( fin ) -> tm 
     | tVoid   => congr_tVoid 
     | tAbsurd  s0 => congr_tAbsurd ((compSubstSubst_tm sigmatm tautm thetatm Eqtm) s0)
     | tEq  s0 s1 s2 s3 => congr_tEq eq_refl ((compSubstSubst_tm sigmatm tautm thetatm Eqtm) s1) ((compSubstSubst_tm sigmatm tautm thetatm Eqtm) s2) ((compSubstSubst_tm sigmatm tautm thetatm Eqtm) s3)
-    | tJ  s0 s1 s2 => congr_tJ ((compSubstSubst_tm (up_tm_tm (up_tm_tm sigmatm)) (up_tm_tm (up_tm_tm tautm)) (up_tm_tm (up_tm_tm thetatm)) (up_subst_subst_tm_tm (_) (_) (_) (up_subst_subst_tm_tm (_) (_) (_) Eqtm))) s0) ((compSubstSubst_tm sigmatm tautm thetatm Eqtm) s1) ((compSubstSubst_tm sigmatm tautm thetatm Eqtm) s2)
+    | tJ  s0 s1 => congr_tJ ((compSubstSubst_tm sigmatm tautm thetatm Eqtm) s0) ((compSubstSubst_tm sigmatm tautm thetatm Eqtm) s1)
     | tRefl   => congr_tRefl 
     | tSig  s0 s1 s2 => congr_tSig eq_refl ((compSubstSubst_tm sigmatm tautm thetatm Eqtm) s1) ((compSubstSubst_tm (up_tm_tm sigmatm) (up_tm_tm tautm) (up_tm_tm thetatm) (up_subst_subst_tm_tm (_) (_) (_) Eqtm)) s2)
     | tPack  s0 s1 s2 => congr_tPack eq_refl ((compSubstSubst_tm sigmatm tautm thetatm Eqtm) s1) ((compSubstSubst_tm sigmatm tautm thetatm Eqtm) s2)
@@ -274,7 +274,7 @@ Fixpoint rinst_inst_tm   (xitm : ( fin ) -> fin) (sigmatm : ( fin ) -> tm ) (Eqt
     | tVoid   => congr_tVoid 
     | tAbsurd  s0 => congr_tAbsurd ((rinst_inst_tm xitm sigmatm Eqtm) s0)
     | tEq  s0 s1 s2 s3 => congr_tEq eq_refl ((rinst_inst_tm xitm sigmatm Eqtm) s1) ((rinst_inst_tm xitm sigmatm Eqtm) s2) ((rinst_inst_tm xitm sigmatm Eqtm) s3)
-    | tJ  s0 s1 s2 => congr_tJ ((rinst_inst_tm (upRen_tm_tm (upRen_tm_tm xitm)) (up_tm_tm (up_tm_tm sigmatm)) (rinstInst_up_tm_tm (_) (_) (rinstInst_up_tm_tm (_) (_) Eqtm))) s0) ((rinst_inst_tm xitm sigmatm Eqtm) s1) ((rinst_inst_tm xitm sigmatm Eqtm) s2)
+    | tJ  s0 s1 => congr_tJ ((rinst_inst_tm xitm sigmatm Eqtm) s0) ((rinst_inst_tm xitm sigmatm Eqtm) s1)
     | tRefl   => congr_tRefl 
     | tSig  s0 s1 s2 => congr_tSig eq_refl ((rinst_inst_tm xitm sigmatm Eqtm) s1) ((rinst_inst_tm (upRen_tm_tm xitm) (up_tm_tm sigmatm) (rinstInst_up_tm_tm (_) (_) Eqtm)) s2)
     | tPack  s0 s1 s2 => congr_tPack eq_refl ((rinst_inst_tm xitm sigmatm Eqtm) s1) ((rinst_inst_tm xitm sigmatm Eqtm) s2)
